Test_ReTierStaticSemantics.v
@@ -16,14 +16,15 @@ Require Import ReTierSyntax.
 **)
 
 
-Definition testPsi1: reactEnv   := reactUpdate (Reactive 0) Unit reactEmpty.
-Definition testGamma1: varEnv   := idUpdate (Id "x") Tnat (idUpdate (Id "y") Unit idEmpty).
+Definition testPsi0: reactiveEnv := Datatypes.nil.
+Definition testPsi1: reactiveEnv := Datatypes.cons Unit Datatypes.nil.
+Definition testGamma1: varEnv := idUpdate (Id "x") Tnat (idUpdate (Id "y") Unit idEmpty).
 Definition testDelta1: placeEnv := idUpdate (Id "x") (Unit on (Peer "px")) idEmpty.
-Definition testTies1  := Ties ["p0" -*-> "pm", "p0" -?-> "po", "p0" -1-> "ps", "p0" -0-> "pn"].
+Definition testTies1 := Ties ["p0" -*-> "pm", "p0" -?-> "po", "p0" -1-> "ps", "p0" -0-> "pn"].
 Definition testPeerTyping1 := TypedInstances [4 : "pm", 3 : "po", 2 : "ps", 1 : "pn", 0 : "p0"].
 
 Example test_pltIsWellTyped_TEnd_1:
-  (Program NoTies NoTypedInstances) :: emptyReactEnv; emptyPlaceEnv |- pUnit.
+  (Program NoTies NoTypedInstances) :: testPsi0; emptyPlaceEnv |- pUnit.
 Proof. apply T_End. Qed.
 
 
@@ -33,7 +34,7 @@ Proof. apply T_End. Qed.
 
 
 Example test_hasType_TUnit_1:
-  (Program NoTies NoTypedInstances) :: emptyReactEnv; emptyPlaceEnv; emptyVarEnv; Peer "dummy" |- unit : Unit.
+  (Program NoTies NoTypedInstances) :: testPsi0; emptyPlaceEnv; emptyVarEnv; Peer "dummy" |- unit : Unit.
 Proof. apply T_Unit. Qed.
 
 
@@ -47,33 +48,33 @@ Qed.
 
 
 Example test_hasType_TVar_normalVar_1:
-  (Program NoTies NoTypedInstances) :: emptyReactEnv; emptyPlaceEnv; testGamma1; Peer "p1" |- idApp (Id "x") : Tnat.
+  (Program NoTies NoTypedInstances) :: testPsi0; emptyPlaceEnv; testGamma1; Peer "p1" |- idApp (Id "x") : Tnat.
 Proof. apply T_Var. left. reflexivity. Qed.
 
 
 Example test_hasType_TVar_placedVar_2:
-  (Program NoTies NoTypedInstances) :: emptyReactEnv; testDelta1; emptyVarEnv; Peer "px" |- idApp (Id "x") : Unit.
+  (Program NoTies NoTypedInstances) :: testPsi0; testDelta1; emptyVarEnv; Peer "px" |- idApp (Id "x") : Unit.
 Proof. apply T_Var. right. split. - reflexivity. - reflexivity. Qed.
 
 
 Example test_hasType_TAbs_1: 
-    (Program NoTies NoTypedInstances) :: emptyReactEnv; emptyPlaceEnv; emptyVarEnv; Peer "dummy" |- lambda (Id "x") Tnat unit : Tnat ~> Unit.
+    (Program NoTies NoTypedInstances) :: testPsi0; emptyPlaceEnv; emptyVarEnv; Peer "dummy" |- lambda (Id "x") Tnat unit : Tnat ~> Unit.
 Proof. apply T_Abs. apply T_Unit. Qed.
 
 
 Example test_hasType_TAbs_2: 
-    (Program NoTies NoTypedInstances) :: emptyReactEnv; emptyPlaceEnv; emptyVarEnv; Peer "dummy" |- lambda (Id "x") Tnat (idApp (Id "x")) : Tnat ~> Tnat.
+    (Program NoTies NoTypedInstances) :: testPsi0; emptyPlaceEnv; emptyVarEnv; Peer "dummy" |- lambda (Id "x") Tnat (idApp (Id "x")) : Tnat ~> Tnat.
 Proof. apply T_Abs. apply T_Var. left. reflexivity. Qed.
 
 
 (** Tests variable shadowing **)
 Example test_hasType_TAbs_3:
-  (Program NoTies NoTypedInstances) :: emptyReactEnv; emptyPlaceEnv; testGamma1; Peer "_" |- lambda (Id "x") Unit (idApp (Id "x")) : Unit ~> Unit.
+  (Program NoTies NoTypedInstances) :: testPsi0; emptyPlaceEnv; testGamma1; Peer "_" |- lambda (Id "x") Unit (idApp (Id "x")) : Unit ~> Unit.
 Proof. apply T_Abs. apply T_Var. left. reflexivity. Qed.
 
 
 Example test_hasType_TApp_1:
-  (Program NoTies NoTypedInstances) :: emptyReactEnv; emptyPlaceEnv; emptyVarEnv; Peer "dummy" |- app (lambda (Id "x") Unit unit) unit : Unit.
+  (Program NoTies NoTypedInstances) :: testPsi0; emptyPlaceEnv; emptyVarEnv; Peer "dummy" |- app (lambda (Id "x") Unit unit) unit : Unit.
 Proof.
   apply T_App with (T2 := Unit).
   - apply T_Abs. apply T_Unit.
@@ -82,7 +83,7 @@ Qed.
 
 
 Example test_hasType_TApp_2: 
-  (Program NoTies NoTypedInstances) :: emptyReactEnv; emptyPlaceEnv; emptyVarEnv; Peer "dummy" |- app (lambda (Id "x") Unit (idApp (Id "x"))) unit : Unit.
+  (Program NoTies NoTypedInstances) :: testPsi0; emptyPlaceEnv; emptyVarEnv; Peer "dummy" |- app (lambda (Id "x") Unit (idApp (Id "x"))) unit : Unit.
 Proof.
   apply T_App with (T2 := Unit).
   - apply T_Abs. apply T_Var. left. reflexivity.
@@ -91,12 +92,12 @@ Qed.
 
 
 Example test_hasType_TNil_1: 
-  (Program NoTies NoTypedInstances) :: emptyReactEnv; emptyPlaceEnv; emptyVarEnv; Peer "dummy" |- nil Unit : List Unit.
+  (Program NoTies NoTypedInstances) :: testPsi0; emptyPlaceEnv; emptyVarEnv; Peer "dummy" |- nil Unit : List Unit.
 Proof. apply T_Nil. Qed.
 
 
 Example test_hasType_TCons_1: 
-  (Program NoTies NoTypedInstances) :: emptyReactEnv; emptyPlaceEnv; emptyVarEnv; Peer "dummy" |- cons unit (nil Unit) : List Unit.
+  (Program NoTies NoTypedInstances) :: testPsi0; emptyPlaceEnv; emptyVarEnv; Peer "dummy" |- cons unit (nil Unit) : List Unit.
 Proof.
   apply T_Cons.
   - apply T_Unit.
@@ -105,17 +106,17 @@ Qed.
 
 
 Example test_hasType_TSome_1: 
-    (Program NoTies NoTypedInstances) :: emptyReactEnv; emptyPlaceEnv; emptyVarEnv; Peer "dummy" |- some unit : Option Unit.
+    (Program NoTies NoTypedInstances) :: testPsi0; emptyPlaceEnv; emptyVarEnv; Peer "dummy" |- some unit : Option Unit.
 Proof. apply T_Some. apply T_Unit. Qed.
 
 
 Example test_hasType_TNone_1: 
-    (Program NoTies NoTypedInstances) :: emptyReactEnv; emptyPlaceEnv; emptyVarEnv; Peer "dummy" |- none Unit : Option Unit.
+    (Program NoTies NoTypedInstances) :: testPsi0; emptyPlaceEnv; emptyVarEnv; Peer "dummy" |- none Unit : Option Unit.
 Proof. apply T_None. Qed.
 
 
 Example test_hasType_TPeer_1:
-  (Program testTies1 testPeerTyping1) :: emptyReactEnv; emptyPlaceEnv; emptyVarEnv; Peer "p0" |- peerApp (PeerInstance 0) : Remote (Peer "p0").
+  (Program testTies1 testPeerTyping1) :: testPsi0; emptyPlaceEnv; emptyVarEnv; Peer "p0" |- peerApp (PeerInstance 0) : Remote (Peer "p0").
 Proof. apply T_Peer. reflexivity. Qed.
 
 
@@ -123,7 +124,7 @@ Example test_hasType_TAsLocal_single_1:
   (* ensure test setup is correct ... *)
   testTies1 (Peer "p0", Peer "ps") = Single /\
   (* actual test ... *)
-  (Program testTies1 NoTypedInstances) :: emptyReactEnv; emptyPlaceEnv; emptyVarEnv; Peer "p0"
+  (Program testTies1 NoTypedInstances) :: testPsi0; emptyPlaceEnv; emptyVarEnv; Peer "p0"
     |- asLocal unit (Unit on (Peer "ps")) : Unit.
 Proof.
   split.
@@ -140,7 +141,7 @@ Example test_hasType_TAsLocal_optional_1:
   (* ensure test setup is correct ... *)
   testTies1 (Peer "p0", Peer "po") = Optional /\
   (* actual test ... *)
-  (Program testTies1 NoTypedInstances) :: emptyReactEnv; emptyPlaceEnv; emptyVarEnv; Peer "p0"
+  (Program testTies1 NoTypedInstances) :: testPsi0; emptyPlaceEnv; emptyVarEnv; Peer "p0"
     |- asLocal unit (Unit on (Peer "po")) : Option Unit.
 Proof.
   split.
@@ -157,7 +158,7 @@ Example test_hasType_TAsLocal_multiple_1:
   (* ensure test setup is correct ... *)
   testTies1 (Peer "p0", Peer "pm") = Multiple /\
   (* actual test ... *)
-  (Program testTies1 NoTypedInstances) :: emptyReactEnv; emptyPlaceEnv; emptyVarEnv; Peer "p0"
+  (Program testTies1 NoTypedInstances) :: testPsi0; emptyPlaceEnv; emptyVarEnv; Peer "p0"
     |- asLocal unit (Unit on (Peer "pm")) : List Unit.
 Proof.
   split.
@@ -175,7 +176,7 @@ Example test_hasType_TAsLocalFrom_single_1:
   typed_peer_instances_type testPeerTyping1 (PeerInstance 2) = Some (Peer "ps") /\
   testTies1 (Peer "p0", Peer "ps") = Single /\
   (* actual test ... *)
-  (Program testTies1 testPeerTyping1) :: emptyReactEnv; emptyPlaceEnv; emptyVarEnv; Peer "p0"
+  (Program testTies1 testPeerTyping1) :: testPsi0; emptyPlaceEnv; emptyVarEnv; Peer "p0"
     |- asLocalFrom unit (Unit on (Peer "ps")) (peerApp (PeerInstance 2)) : Unit.
 Proof.
   split.
@@ -195,7 +196,7 @@ Example test_hasType_TAsLocalFrom_optional_1:
   typed_peer_instances_type testPeerTyping1 (PeerInstance 3) = Some (Peer "po") /\
   testTies1 (Peer "p0", Peer "po") = Optional /\
   (* actual test ... *)
-  (Program testTies1 testPeerTyping1) :: emptyReactEnv; emptyPlaceEnv; emptyVarEnv; Peer "p0"
+  (Program testTies1 testPeerTyping1) :: testPsi0; emptyPlaceEnv; emptyVarEnv; Peer "p0"
     |- asLocalFrom unit (Unit on (Peer "po")) (peerApp (PeerInstance 3)) : Unit.
 Proof.
   split.
@@ -215,7 +216,7 @@ Example test_hasType_TAsLocalFrom_multiple_1:
   typed_peer_instances_type testPeerTyping1 (PeerInstance 4) = Some (Peer "pm") /\
   testTies1 (Peer "p0", Peer "pm") = Multiple /\
   (* actual test ... *)
-  (Program testTies1 testPeerTyping1) :: emptyReactEnv; emptyPlaceEnv; emptyVarEnv; Peer "p0"
+  (Program testTies1 testPeerTyping1) :: testPsi0; emptyPlaceEnv; emptyVarEnv; Peer "p0"
     |- asLocalFrom unit (Unit on (Peer "pm")) (peerApp (PeerInstance 4)) : Unit.
 Proof.
   split.
@@ -234,7 +235,7 @@ Example test_hasType_TComp_single_1:
   (* ensure test setup is correct ... *)
   testTies1 (Peer "p0", Peer "ps") = Single /\
   (* actual test ... *)
-  (Program testTies1 NoTypedInstances) :: emptyReactEnv; emptyPlaceEnv; emptyVarEnv; Peer "p0"
+  (Program testTies1 NoTypedInstances) :: testPsi0; emptyPlaceEnv; emptyVarEnv; Peer "p0"
     |- asLocalIn (Id "x") unit unit (Unit on (Peer "ps")) : Unit.
 Proof.
   split.
@@ -253,7 +254,7 @@ Example test_hasType_TComp_optional_1:
   (* ensure test setup is correct ... *)
   testTies1 (Peer "p0", Peer "po") = Optional /\
   (* actual test ... *)
-  (Program testTies1 NoTypedInstances) :: emptyReactEnv; emptyPlaceEnv; emptyVarEnv; Peer "p0"
+  (Program testTies1 NoTypedInstances) :: testPsi0; emptyPlaceEnv; emptyVarEnv; Peer "p0"
     |- asLocalIn (Id "x") unit unit (Unit on (Peer "po")) : Option Unit.
 Proof.
   split.
@@ -272,7 +273,7 @@ Example test_hasType_TComp_multiple_1:
   (* ensure test setup is correct ... *)
   testTies1 (Peer "p0", Peer "pm") = Multiple /\
   (* actual test ... *)
-  (Program testTies1 NoTypedInstances) :: emptyReactEnv; emptyPlaceEnv; emptyVarEnv; Peer "p0"
+  (Program testTies1 NoTypedInstances) :: testPsi0; emptyPlaceEnv; emptyVarEnv; Peer "p0"
     |- asLocalIn (Id "x") unit unit (Unit on (Peer "pm")) : List Unit.
 Proof.
   split.
@@ -291,7 +292,7 @@ Example test_hasType_TComp_single_2:
   (* ensure test setup is correct ... *)
   testTies1 (Peer "p0", Peer "ps") = Single /\
   (* actual test ... *)
-  (Program testTies1 NoTypedInstances) :: emptyReactEnv; emptyPlaceEnv; emptyVarEnv; Peer "p0"
+  (Program testTies1 NoTypedInstances) :: testPsi0; emptyPlaceEnv; emptyVarEnv; Peer "p0"
     |- asLocalIn (Id "x") unit (idApp (Id "x")) (Unit on (Peer "ps")) : Unit.
 Proof.
   split.
@@ -311,7 +312,7 @@ Example test_hasType_TCompFrom_single_1:
   typed_peer_instances_type testPeerTyping1 (PeerInstance 2) = Some (Peer "ps") /\
   testTies1 (Peer "p0", Peer "ps") = Single /\
   (* actual test ... *)
-  (Program testTies1 testPeerTyping1) :: emptyReactEnv; emptyPlaceEnv; emptyVarEnv; Peer "p0"
+  (Program testTies1 testPeerTyping1) :: testPsi0; emptyPlaceEnv; emptyVarEnv; Peer "p0"
     |- asLocalInFrom (Id "x") (*=*) unit (*in*) unit (*:*) (Unit on (Peer "ps"))
                      (*from*) (peerApp (PeerInstance 2))
     : Unit.
@@ -335,7 +336,7 @@ Example test_hasType_TCompFrom_single_2:
   typed_peer_instances_type testPeerTyping1 (PeerInstance 2) = Some (Peer "ps") /\
   testTies1 (Peer "p0", Peer "ps") = Single /\
   (* actual test ... *)
-  (Program testTies1 testPeerTyping1) :: emptyReactEnv; emptyPlaceEnv; emptyVarEnv; Peer "p0"
+  (Program testTies1 testPeerTyping1) :: testPsi0; emptyPlaceEnv; emptyVarEnv; Peer "p0"
     |- asLocalInFrom (Id "x") (*=*) unit (*in*) (idApp (Id "x"))
                      (*:*) (Unit on (Peer "ps"))
                      (*from*) (peerApp (PeerInstance 2))
@@ -357,7 +358,7 @@ Qed.
 
 Example test_hasType_TReactive_1:
   (* ensure test setup is correct ... *)
-  testPsi1 (Reactive 0) = Some Unit /\
+  reactive_type (Reactive 0) testPsi1 = Some Unit /\
   (* actual test ... *)
   (Program NoTies NoTypedInstances) :: testPsi1; emptyPlaceEnv; emptyVarEnv; Peer "_" |- reactApp (Reactive 0) : Unit.
 Proof.
@@ -368,17 +369,17 @@ Qed.
 
 
 Example test_hasType_TSignal_1:
-  (Program NoTies NoTypedInstances) :: emptyReactEnv; emptyPlaceEnv; emptyVarEnv; Peer "dummy" |- signal unit : Signal Unit.
+  (Program NoTies NoTypedInstances) :: testPsi0; emptyPlaceEnv; emptyVarEnv; Peer "dummy" |- signal unit : Signal Unit.
 Proof. apply T_Signal. apply T_Unit. Qed.
 
 
 Example test_hasType_TReactiveVal_1:
-  (Program NoTies NoTypedInstances) :: emptyReactEnv; emptyPlaceEnv; emptyVarEnv; Peer "dummy" |- var unit : Var Unit.
+  (Program NoTies NoTypedInstances) :: testPsi0; emptyPlaceEnv; emptyVarEnv; Peer "dummy" |- var unit : Var Unit.
 Proof. apply T_ReactiveVar. apply T_Unit. Qed.
 
 
 Example test_hasType_TNow_signal_1:
-  (Program NoTies NoTypedInstances) :: emptyReactEnv; emptyPlaceEnv; emptyVarEnv; Peer "dummy" |- now (signal unit) : Unit.
+  (Program NoTies NoTypedInstances) :: testPsi0; emptyPlaceEnv; emptyVarEnv; Peer "dummy" |- now (signal unit) : Unit.
 Proof.
   apply T_Now with (T0 := Signal Unit).
   - apply T_Signal. apply T_Unit.
@@ -387,7 +388,7 @@ Qed.
 
 
 Example test_hasType_TNow_var_1:
-  (Program NoTies NoTypedInstances) :: emptyReactEnv; emptyPlaceEnv; emptyVarEnv; Peer "dummy" |- now (var unit) : Unit.
+  (Program NoTies NoTypedInstances) :: testPsi0; emptyPlaceEnv; emptyVarEnv; Peer "dummy" |- now (var unit) : Unit.
 Proof.
   eapply T_Now.
   - apply T_ReactiveVar. apply T_Unit.
@@ -396,7 +397,7 @@ Qed.
 
 
 Example test_hasType_TSet_1:
-  (Program NoTies NoTypedInstances) :: emptyReactEnv; emptyPlaceEnv; emptyVarEnv; Peer "dummy" |- set (var unit) unit : Unit.
+  (Program NoTies NoTypedInstances) :: testPsi0; emptyPlaceEnv; emptyVarEnv; Peer "dummy" |- set (var unit) unit : Unit.
 Proof.
   apply T_Set with (T := Unit).
   - apply T_ReactiveVar. apply T_Unit.
@@ -405,12 +406,12 @@ Qed.
 
 
 Example test_hasType_TSet_2:
-  (Program NoTies NoTypedInstances) :: emptyReactEnv; emptyPlaceEnv; emptyVarEnv; Peer "dummy"
+  (Program NoTies NoTypedInstances) :: testPsi0; emptyPlaceEnv; emptyVarEnv; Peer "dummy"
     |- set (var (lambda (Id "x") Unit unit))
            (*:=*) (lambda (Id "x") Unit unit)
     : Unit.
 Proof.
-  assert (H: (Program NoTies NoTypedInstances) :: emptyReactEnv; emptyPlaceEnv; emptyVarEnv; Peer "dummy" |- lambda (Id "x") Unit unit : Unit ~> Unit).
+  assert (H: (Program NoTies NoTypedInstances) :: testPsi0; emptyPlaceEnv; emptyVarEnv; Peer "dummy" |- lambda (Id "x") Unit unit : Unit ~> Unit).
   - apply T_Abs.
     apply T_Unit.
   - apply T_Set with (T := Unit ~> Unit).
